Investigating the Soundness theorem

sitpn2hvhdl/Soundness.v
@@ -48,8 +48,24 @@ Definition EnvEq sitpn (Ec : nat -> C sitpn -> bool) (Ep : nat -> Clk -> IdMap v
     a H-VHDL design state.
  *)
 
-Definition SimState {sitpn} (s : SitpnState sitpn) (σ : DState) : Prop := False.
-Local Notation "s '∼' σ" := (SimState s σ) (at level 50).
+Definition SimState {sitpn} (γ : P sitpn + T sitpn -> ident) (s : SitpnState sitpn) (σ : DState) : Prop :=
+
+  (* Markings are similar. *)
+  
+  forall (p : P sitpn) id__p σ__p,
+    (* [idp] is the identifier of the place component associated with
+       place [p] by the [γ] binder. *)
+    γ (inl p) = id__p ->
+
+    (* [σp] is the current state of component [idp] is the global design
+       state [σ]. *)
+    MapsTo id__p σ__p (compstore σ) ->
+
+    (* Marking of place [p] at state [s] equals value of signal
+       [s_marking] at state [σp]. *)
+    MapsTo Place.s_marking (Vnat (M s p)) (sigstore σ__p).
+
+Local Notation "γ ⊢ s '∼' σ" := (SimState γ s σ) (at level 50).
 
 (** States that two execution trace are similar. The first list
     argument is the execution trace of an SITPN and the second list
@@ -58,12 +74,153 @@ Local Notation "s '∼' σ" := (SimState s σ) (at level 50).
     By construction, and in order to be similar, the two traces must
     have the same length, and must have pair-wise similar states. *)
 
-Inductive SimTrace {sitpn} : list (SitpnState sitpn) -> list DState -> Prop :=
-| SimTraceInit: SimTrace nil nil
+Inductive SimTrace {sitpn} γ : list (SitpnState sitpn) -> list DState -> Prop :=
+| SimTraceInit: SimTrace γ nil nil
 | SimTraceCons: forall s σ θ__s θ__σ,
-    s ∼ σ ->
-    SimTrace θ__s θ__σ ->
-    SimTrace (s :: θ__s) (σ :: θ__σ).
+    γ ⊢ s ∼ σ ->
+    SimTrace γ θ__s θ__σ ->
+    SimTrace γ (s :: θ__s) (σ :: θ__σ).
+
+(** ** Rising edge marking equal lemma
+
+    States that starting from similar state, markings are equal
+    after the rising edge of the clock signal.  *)
+
+Lemma rising_edge_marking_equal :
+  forall Δ σ__r d θ σ' σ sitpn Ec τ s s' mm γ,
+
+    (* sitpn translates into d. *)
+    sitpn_to_hvhdl sitpn mm = Success d ->
+
+    (* Similar starting states *)
+    γ ⊢ s ∼ σ ->
+    
+    (* Rising edge from s to s', s ⇝↑ s' *)
+    SitpnStateTransition Ec τ s s' rising_edge -> 
+
+    (* Rising edge from σ to σr *)
+    vrising Δ σ (get_behavior d) σ__r -> 
+
+    (* Stabilize from σr to σ' *)
+    stabilize Δ σ__r (get_behavior d) θ σ' ->
+    
+    (* Conclusion *)
+    forall p id__p σ'__p,
+      (* [idp] is the identifier of the place component associated with
+       place [p] by the [γ] binder. *)
+      γ (inl p) = id__p ->
+
+      (* [σp] is the current state of component [idp] is the global design
+       state [σ]. *)
+      MapsTo id__p σ'__p (compstore σ') ->
+
+      (* Marking of place [p] at state [s] equals value of signal
+         [s_marking] at state [σp]. *)
+      MapsTo Place.s_marking (Vnat (@M sitpn s' p)) (sigstore σ'__p).
+Proof.
+Admitted.
+
+(** ** Rising edge states equal.
+ 
+    Utopic lemma; not sure it is provable. *)
+
+Lemma rising_edge_states_equal :
+  forall Δ σ__r d θ σ' σ sitpn E__c τ s s' mm (γ : P sitpn + T sitpn -> ident),
+
+    (* sitpn translates into d. *)
+    sitpn_to_hvhdl sitpn mm = Success d ->
+
+    (* Similar starting states *)
+    γ ⊢ s ∼ σ ->
+    
+    (* Rising edge from s to s', s ⇝↑ s' *)
+    SitpnStateTransition E__c τ s s' rising_edge -> 
+
+    (* Rising edge from σ to σr *)
+    vrising Δ σ (get_behavior d) σ__r -> 
+
+    (* Stabilize from σr to σ' *)
+    stabilize Δ σ__r (get_behavior d) θ σ' ->
+    
+    (* Conclusion *)
+    γ ⊢ s' ∼ σ'.
+Proof.
+Admitted.
+
+(** ** Falling edge compute fired lemma
+
+    States that starting from similar state, after the falling edge of
+    the clock signal, all fired transitions are associated with
+    transition components with a fired out port valuated to true (or
+    false otherwise).  *)
+
+Lemma falling_edge_compute_fired :
+  forall Δ σ__f d θ σ' σ sitpn Ec τ s s' mm γ id__t σ'__t,
+
+    (* sitpn translates into d. *)
+    sitpn_to_hvhdl sitpn mm = Success d ->
+
+    (* Similar starting states *)
+    γ ⊢ s ∼ σ ->
+    
+    (* Falling edge from s to s', s ⇝↓ s' *)
+    SitpnStateTransition Ec τ s s' falling_edge -> 
+
+    (* Falling edge from σ to σf *)
+    vfalling Δ σ (get_behavior d) σ__f -> 
+
+    (* Stabilize from σf to σ' *)
+    stabilize Δ σ__f (get_behavior d) θ σ' ->
+    
+    (* Conclusion *)
+    forall fset t,
+      (** Component idt implements transition t *)
+      γ (inr t) = id__t ->
+
+      (* σ't is the state of component idt at design's state σ'. *)
+      MapsTo id__t σ'__t (compstore σ') ->
+
+      (* Conclusion *)
+      @Fired sitpn s' fset t ->
+      MapsTo Transition.fired (Vbool true) (sigstore σ'__t).
+Proof.
+  intros.
+  unfold Fired in H6.
+  induction H6.
+  inversion H6.
+  inversion_clear H9.
+  - admit.
+  - unfold SitpnSemanticsDefs.Set_in_List in H8.
+    induction H8.
+    generalize (H8 t).
+Admitted.  
+
+(** ** Falling edge states equal.
+ 
+    Utopic lemma; not sure it is provable. *)
+
+Lemma falling_edge_states_equal :
+  forall Δ σ__f d θ σ' σ sitpn Ec τ s s' mm (γ : P sitpn + T sitpn -> ident),
+
+    (* sitpn translates into d. *)
+    sitpn_to_hvhdl sitpn mm = Success d ->
+
+    (* Similar starting states *)
+    γ ⊢ s ∼ σ ->
+    
+    (* Falling edge from s to s', s ⇝↓ s' *)
+    SitpnStateTransition Ec τ s s' falling_edge -> 
+
+    (* Falling edge from σ to σf *)
+    vfalling Δ σ (get_behavior d) σ__f -> 
+
+    (* Stabilize from σf to σ' *)
+    stabilize Δ σ__f (get_behavior d) θ σ' ->
+
+    (* Conclusion *)
+    γ ⊢ s' ∼ σ'.
+Proof.
+Admitted.
 
 (** ** Step lemma
     
@@ -73,13 +230,13 @@ Inductive SimTrace {sitpn} : list (SitpnState sitpn) -> list DState -> Prop :=
  *)
 
 Lemma step_lemma :
-  forall sitpn mm d s s' E__c σ σ' Δ Mg σ__e P__i τ,
+  forall sitpn mm d s s' E__c σ σ' Δ Mg σ__e P__i τ γ,
     
     (* sitpn translates into d. *)
     sitpn_to_hvhdl sitpn mm = Success d ->
 
     (* Starting states are similar *)
-    s ∼ σ ->
+    γ ⊢ s ∼ σ ->
 
     (* Δ, σ are the results of the elaboration of d. *)
     edesign hdstore Mg d Δ σ__e ->
@@ -92,15 +249,38 @@ Lemma step_lemma :
     simcycle P__i Δ τ σ (get_behavior d) σ' ->
      
     (* Final states are similar *)
-    s' ∼ σ'.
+    γ ⊢ s' ∼ σ'.
 Proof.
+  intros *; intros Htransl Hsim Helab Hsitpn_cyc Hhdl_cyc.
+  unfold SitpnCycle in Hsitpn_cyc.
+  inversion_clear Hsitpn_cyc as (s__i & (Hrising, Hfalling)).
+  inversion_clear Hhdl_cyc as
+      (σ__injr, σ__r, σ__i, σ__injf, σ__f, σ'', θ, θ',
+       Hhdl_rising, Hstab_rising, Hhdl_falling, Hstab_falling, Hinj_rising, Hinj_falling).
+
+  (* Must prove s similar to σ after capture of input values on rising edge. 
+     Necessary premise to apply [rising_edge_states_equal].      
+   *)
+  cut (γ ⊢ s ∼ σ__injr); intros Hsim_injr.
+  specialize (rising_edge_states_equal
+           Δ σ__r d θ σ__i σ__injr sitpn E__c τ s s__i mm γ
+           Htransl Hsim_injr Hrising Hhdl_rising Hstab_rising); intros Heq_int_states.
+
+  (* Must prove s similar to σ after capture of input values on falling edge. 
+     Necessary premise to apply [falling_edge_states_equal].
+   *)
+  cut (γ ⊢ s__i ∼ σ__injf); intros Hsim_injf.
+  apply (falling_edge_states_equal Δ σ__f d θ' σ' σ__injf sitpn E__c τ s__i s' mm γ
+                                   Htransl Hsim_injf Hfalling Hhdl_falling Hstab_falling).
   
+  - admit.
+  - admit.
 Admitted.
 
 (** ** Equal Initial States  *)
 
 Lemma init_states_sim :
-  forall sitpn mm d Mg Δ σ__e σ0,
+  forall sitpn mm d Mg Δ σ__e σ0 γ,
     
     (* sitpn translates into d. *)
     sitpn_to_hvhdl sitpn mm = Success d ->
@@ -112,12 +292,13 @@ Lemma init_states_sim :
     init Δ σ__e (get_behavior d) σ0 ->
 
     (* init states are similar *)
-    (s0 sitpn) ∼ σ0.
+    γ ⊢ (s0 sitpn) ∼ σ0.
 Proof.
   intros *; intros Htransl Helab Hinit.
-  inversion_clear Hinit as (σ', beh, σ, σ'', θ, Hruninit, Hstab).
-Admitted.
+  inversion_clear Hinit as (σ, beh, σ', σ'', θ, Hruninit, Hstab).
 
+Admitted.
+  
 (** ** Simulation Lemma *)
 
 Lemma simulation_lemma :
@@ -128,7 +309,7 @@ Lemma simulation_lemma :
        producing trace θs. *)
     SitpnExecute Ec s τ θ__s s' ->
 
-    forall d mm Ep Mg Δ σ__e θ__σ σ σ',
+    forall d mm Ep Mg Δ σ__e θ__σ σ σ' γ,
       
     (* sitpn translates into d. *)
     sitpn_to_hvhdl sitpn mm = Success d ->
@@ -140,13 +321,13 @@ Lemma simulation_lemma :
     edesign hdstore Mg d Δ σ__e ->
 
     (* States s and σ are similar; *)
-    s ∼ σ ->
+    γ ⊢ s ∼ σ ->
     
     (* From σ to σ' after τ execution cycles, producing trace θσ. *)
     simloop Ep Δ σ (get_behavior d) τ θ__σ σ' ->
 
     (* Conclusion *)
-    SimTrace θ__s θ__σ.
+    SimTrace γ θ__s θ__σ.
 Proof.
   intros *; intros Hexec; dependent induction Hexec;
   intros *; intros Htransl Henveq Helab Hsimstate Hsim.
@@ -160,23 +341,24 @@ Proof.
     (* Specializes the induction hypothesis, then apply the step lemma. *)
     
     specialize (IHHexec d mm Ep Mg Δ σ__e θ0 σ0 σ').
-    specialize (IHHexec Htransl Henveq Helab).
+    specialize (IHHexec γ Htransl Henveq Helab).
 
     (* Then, we need a lemma stating that s' ∼ σ0. That is, state are
        similar after one execution cycle. *)
 
-    specialize (step_lemma sitpn mm d s s' Ec σ σ0 Δ Mg σ__e Ep (S tau)
+    specialize (step_lemma sitpn mm d s s' Ec σ σ0 Δ Mg σ__e Ep (S tau) γ
                            Htransl Hsimstate Helab H Hcyc)
       as Heq_state_cyc.
 
     (* Solve the induction case. *)
-    apply SimTraceCons; [ assumption | apply (IHHexec Heq_state_cyc Hsiml)].
+    apply (@SimTraceCons sitpn γ s' σ0 θ θ0);
+      [ assumption | apply (IHHexec Heq_state_cyc Hsiml)].
 Qed.
 
 (** ** Semantic Preservation Theorem *)
 
 Theorem sitpn2vhdl_sound :
-  forall sitpn E__c τ θ__s s' d Mg E__p σ' mm Δ σ__e σ0 θ__σ,
+  forall sitpn E__c τ θ__s s' d Mg E__p σ' mm Δ σ__e σ0 θ__σ γ,
       
     (* sitpn translates into d. *)
     sitpn_to_hvhdl sitpn mm = Success d ->
@@ -199,7 +381,7 @@ Theorem sitpn2vhdl_sound :
     simloop E__p Δ σ0 (get_behavior d) τ θ__σ σ' ->
     
     (* ** Conclusion: exec. traces are equal. ** *)
-    SimTrace θ__s θ__σ.
+    SimTrace γ θ__s θ__σ.
 Proof.
   intros.
 
@@ -212,50 +394,11 @@ Proof.
     Hinit: init _ _ _ _,
     Hsimloop: simloop _ _ _ _ _ _ _
     |- _ ] =>
-    specialize (init_states_sim sitpn mm d Mg Δ σ__e σ0 Htransl Helab Hinit) as Hinit_eq;
-      apply (simulation_lemma sitpn E__c τ (s0 sitpn) θ__s s' Hsitpnexec
-                              d mm E__p Mg Δ σ__e θ__σ σ0 σ'
-                              Htransl Henveq Helab Hinit_eq Hsimloop)
+    specialize (init_states_sim sitpn mm d Mg Δ σ__e σ0 γ Htransl Helab Hinit) as Hinit_eq;
+      apply (simulation_lemma
+               sitpn E__c τ (s0 sitpn) θ__s s' Hsitpnexec d mm E__p Mg Δ σ__e θ__σ σ0 σ' γ
+               Htransl Henveq Helab Hinit_eq Hsimloop)
   end.
 
 Qed.
     
-Lemma falling_edge_compute_fired :
-  forall Δ σ__f d θ σ' σ sitpn Ec τ s s' mm γ id__t σ'__t,
-
-    (* sitpn translates into d. *)
-    sitpn_to_hvhdl sitpn mm = Success d ->
-
-    (* Similar starting states *)
-    s ∼ σ ->
-
-    (* Falling edge from s to s' *)
-    SitpnStateTransition Ec τ s s' falling_edge ->
-
-    (* Falling edge from σ to σf *)
-    vfalling Δ σ (get_behavior d) σ__f ->
-
-    (* Stabilize from σf to σ' *)
-    stabilize Δ σ__f (get_behavior d) θ σ' ->
-    
-    (* Conclusion *)
-    forall flist t,
-      (** Component idt implements transition t *)
-      γ t = id__t ->
-
-      (* σ't is the state of component idt at design's state σ'. *)
-      MapsTo id__t σ'__t (compstore σ') ->
-
-      (* Conclusion *)
-      @Fired sitpn s' flist t ->
-      MapsTo Transition.fired (Vbool true) (sigstore σ'__t).
-Proof.
-  intros.
-  unfold Fired in H6.
-  inversion H6.
-  inversion H7.
-  inversion H10.
-  - admit.
-  -
-
-Admitted.  
